From10To20/Stmt.v
@@ -1,4 +1,4 @@
-From Coq Require Import String ZArith Eqdep_dec.
+From Coq Require Import String ZArith Eqdep_dec Lia.
 
 From Coq Require PropExtensionality.
 
@@ -42,7 +42,7 @@ Lemma interpret_translated_small_stmt {C: VyperConfig}
                                              do_call_10 fc' world arg_values)
                                 (world: world_state)
                                 (loc: string_map uint256)
-                                {ss10: L10.AST.small_stmt}
+                                (ss10: L10.AST.small_stmt)
                                 {s20: L20.AST.stmt}
                                 (StmtOk: s20 = let is_private_call := fun name: string =>
                                                   match cd_declmap cd name with
@@ -135,8 +135,867 @@ subst. cbn. expr.
 now L10.Expr.destruct_let_pair.
 Qed.
 
-(*
+Ltac mark :=
+  let lhs := fresh "lhs" in
+  let rhs := fresh "rhs" in
+  match goal with
+  |- ?a = ?b => remember a as lhs; remember b as rhs
+  end.
 
+(** Interpreting [head; tail] in L20 is the same as interpreting [head :: tail] in L10. *)
+Local Lemma semicolon_ok {C: VyperConfig}
+                  {bigger_call_depth_bound smaller_call_depth_bound: nat}
+                  (Ebound: bigger_call_depth_bound = S smaller_call_depth_bound)
+                  {cd: L10.Descend.calldag}
+                  (builtins: string -> option builtin)
+                  (fc: fun_ctx cd bigger_call_depth_bound)
+                  {do_call_10: forall
+                        (fc': fun_ctx cd smaller_call_depth_bound)
+                        (world: world_state)
+                        (arg_values: list uint256),
+                      world_state * expr_result uint256}
+                  {do_call_20: forall
+                        (fc': fun_ctx (translate_calldag cd) smaller_call_depth_bound)
+                        (world: world_state)
+                        (arg_values: list uint256),
+                      world_state * expr_result uint256}
+                  (DoCallOk: forall fc' world arg_values,
+                               do_call_20 (translate_fun_ctx fc' eq_refl) world arg_values
+                                =
+                               do_call_10 fc' world arg_values)
+                  (world: world_state)
+                  (loc: string_map uint256)
+                  {head10: L10.AST.stmt}
+                  {tail10: list L10.AST.stmt}
+                  (NotLocalVar: L10.AST.is_local_var_decl head10 = false)
+                  (CallOk20: let _ := string_set_impl in
+                             let is_private_call :=
+                                   fun name: string => match cd_declmap cd name with
+                                                       | Some _ => true
+                                                       | None => false
+                                                       end in
+                               FSet.is_subset
+                                 (Callset.stmt_callset
+                                    (AST.Semicolon
+                                       (translate_stmt is_private_call head10)
+                                       (translate_stmt_list is_private_call tail10)))
+                                 (Callset.decl_callset (fun_decl (translate_fun_ctx fc eq_refl)))
+                               = true)
+                  (HeadCallOk10: let _ := string_set_impl in 
+                     FSet.is_subset (L10.Callset.stmt_callset head10)
+                                    (L10.Callset.decl_callset
+                                      (fun_decl fc))
+                     = true)
+                  (TailCallOk10: let _ := string_set_impl in 
+                     FSet.is_subset (L10.Callset.stmt_list_callset tail10)
+                                    (L10.Callset.decl_callset
+                                      (fun_decl fc))
+                     = true)
+                  (HeadOk:
+                    forall (NotVarDecl: AST.is_local_var_decl head10 = false)
+                           (CallOk20: FSet.is_subset
+                                        (Callset.stmt_callset
+                                           (translate_stmt
+                                              (fun name : string =>
+                                               match cd_declmap cd name with
+                                               | Some _ => true
+                                               | None => false
+                                               end) head10))
+                                        (Callset.decl_callset (cached_translated_decl fc eq_refl))
+                                      = true)
+                           (CallOk10: FSet.is_subset
+                                        (L10.Callset.stmt_callset head10)
+                                        (L10.Callset.decl_callset (fun_decl fc)) = true)
+                           (world: world_state)
+                           (loc: string_map uint256),
+                       Stmt.interpret_stmt Ebound (translate_fun_ctx fc eq_refl) do_call_20 builtins world loc
+                         (translate_stmt
+                            (fun name : string => match cd_declmap cd name with
+                                                  | Some _ => true
+                                                  | None => false
+                                                  end) head10) CallOk20 =
+                       L10.Stmt.interpret_stmt Ebound fc do_call_10 builtins world loc head10 NotVarDecl
+                         CallOk10)
+                  (TailOk: forall (world: world_state) (loc: string_map uint256),
+                    Stmt.interpret_stmt Ebound (translate_fun_ctx fc eq_refl) do_call_20 builtins world loc
+                      (translate_stmt_list
+                         (fun name : string => match cd_declmap cd name with
+                                               | Some _ => true
+                                               | None => false
+                                               end) tail10) (Callset.callset_descend_semicolon_right eq_refl CallOk20) =
+                    Stmt.interpret_stmt_list Ebound fc do_call_10 builtins world loc tail10 TailCallOk10):
+  Stmt.interpret_stmt Ebound (translate_fun_ctx fc eq_refl) do_call_20 builtins world loc
+    (AST.Semicolon
+        (translate_stmt
+           (fun name: string => match cd_declmap cd name with
+                                 | Some _ => true
+                                 | None => false
+                                 end) head10)
+        (translate_stmt_list
+           (fun name: string => match cd_declmap cd name with
+                                 | Some _ => true
+                                 | None => false
+                                 end) tail10))
+    CallOk20
+   =
+  match
+    L10.Stmt.interpret_stmt Ebound fc do_call_10 builtins world loc head10 NotLocalVar HeadCallOk10
+  with
+  | (world', loc', StmtSuccess) =>
+      Stmt.interpret_stmt_list Ebound fc do_call_10 builtins world' loc' tail10 TailCallOk10
+  | (world', loc', StmtAbort _ as result) | (world', loc', StmtReturnFromFunction _ as result) =>
+      (world', loc', result)
+  end.
+Proof.
+cbn.
+rewrite (HeadOk NotLocalVar
+           (Callset.callset_descend_semicolon_left eq_refl CallOk20)
+           HeadCallOk10).
+destruct L10.Stmt.interpret_stmt.
+destruct p as (world', loc').
+destruct s. 2-3:easy.
+apply TailOk.
+Qed.
+
+(* Stmt lists work fine assuming that single stmts work fine. *)
+Local Lemma weak_stmt_list_ok {C: VyperConfig}
+                  {bigger_call_depth_bound smaller_call_depth_bound: nat}
+                  (Ebound: bigger_call_depth_bound = S smaller_call_depth_bound)
+                  {cd: L10.Descend.calldag}
+                  (builtins: string -> option builtin)
+                  (fc: fun_ctx cd bigger_call_depth_bound)
+                  {do_call_10: forall
+                        (fc': fun_ctx cd smaller_call_depth_bound)
+                        (world: world_state)
+                        (arg_values: list uint256),
+                      world_state * expr_result uint256}
+                  {do_call_20: forall
+                        (fc': fun_ctx (translate_calldag cd) smaller_call_depth_bound)
+                        (world: world_state)
+                        (arg_values: list uint256),
+                      world_state * expr_result uint256}
+                  (DoCallOk: forall fc' world arg_values,
+                               do_call_20 (translate_fun_ctx fc' eq_refl) world arg_values
+                                =
+                               do_call_10 fc' world arg_values)
+                  (world: world_state)
+                  (loc: string_map uint256)
+                  {list10: list L10.AST.stmt}
+                  (CallOk20: let _ := string_set_impl in 
+                             let is_private_call := fun name: string =>
+                                      match cd_declmap cd name with
+                                      | Some _ => true
+                                      | _ => false
+                                      end in
+                           FSet.is_subset (L20.Callset.stmt_callset
+                                            (translate_stmt_list is_private_call list10))
+                                          (L20.Callset.decl_callset
+                                             (fun_decl
+                                               (translate_fun_ctx fc eq_refl)))
+                     = true)
+                  (CallOk10: let _ := string_set_impl in 
+                     FSet.is_subset (L10.Callset.stmt_list_callset list10)
+                                    (L10.Callset.decl_callset
+                                      (fun_decl fc))
+                     = true)
+                  (ItemsOk: List.Forall
+                     (fun s: L10.AST.stmt =>
+                        let is_private_call :=
+                          fun name : string => match cd_declmap cd name with
+                                               | Some _ => true
+                                               | None => false
+                                               end in
+                       forall 
+                         (NotVarDecl: AST.is_local_var_decl s = false)
+                         (CallOk20: let H := string_set_impl in
+                                     FSet.is_subset (L20.Callset.stmt_callset (translate_stmt is_private_call s))
+                                       (L20.Callset.decl_callset
+                                         (fun_decl (translate_fun_ctx fc eq_refl))) = true)
+                         (CallOk10: let H := string_set_impl in
+                                     FSet.is_subset (L10.Callset.stmt_callset s)
+                                       (L10.Callset.decl_callset (fun_decl fc)) = true)
+                         (world: world_state)
+                         (loc: string_map uint256),
+                       L20.Stmt.interpret_stmt Ebound (translate_fun_ctx fc eq_refl) do_call_20 builtins world loc
+                          (translate_stmt is_private_call s) CallOk20
+                        =
+                       L10.Stmt.interpret_stmt Ebound fc do_call_10 builtins world loc s NotVarDecl CallOk10)
+                    list10):
+  let is_private_call := fun name: string =>
+                            match cd_declmap cd name with
+                            | Some _ => true
+                            | _ => false
+                            end in
+  L20.Stmt.interpret_stmt Ebound (translate_fun_ctx fc eq_refl) do_call_20 builtins world loc
+    (translate_stmt_list is_private_call list10) CallOk20
+   =
+  L10.Stmt.interpret_stmt_list Ebound fc do_call_10 builtins world loc list10 CallOk10.
+Proof.
+cbn. revert world loc. induction list10; intros. { easy. }
+cbn.
+assert (HeadOk := List.Forall_inv ItemsOk).
+assert (TailOk := List.Forall_inv_tail ItemsOk). 
+clear ItemsOk. cbn in HeadOk.
+pose (is_loc_var := AST.is_local_var_decl a).
+assert (IsLocVar: AST.is_local_var_decl a = is_loc_var) by trivial.
+destruct a;
+  (* this succeeds for everything except loc var decls: *)
+  try rewrite (semicolon_ok Ebound builtins fc DoCallOk world loc IsLocVar
+               CallOk20
+               (Callset.callset_descend_stmt_head eq_refl CallOk10)
+               (Callset.callset_descend_stmt_tail eq_refl CallOk10) 
+               HeadOk
+               (IHlist10 _ _ TailOk));
+  try easy.
+(* local var *)
+cbn. destruct map_lookup. { trivial. }
+destruct init.
+{ (* with init *)
+  expr. destruct L10.Expr.interpret_expr as (w,[result|abort]). 2:trivial.
+  (* why can't I match goal with let '(_, _, _) := ... ? *)
+  remember (L20.Stmt.interpret_stmt _ _ _ _ _ _ _ _) as lhs.
+  remember (Stmt.interpret_stmt_list Ebound fc do_call_10 builtins world 
+                                     (map_insert loc name result) list10
+                                     (Callset.callset_descend_stmt_tail eq_refl CallOk10)) as rhs.
+  assert (G: lhs = rhs). { subst. apply IHlist10. apply TailOk. }
+  now rewrite G.
+}
+(* without init *)
+cbn.
+remember (L20.Stmt.interpret_stmt _ _ _ _ _ _ _ _) as lhs.
+remember (Stmt.interpret_stmt_list Ebound fc do_call_10 builtins world 
+                                   (map_insert loc name zero256) list10
+                                   (Callset.callset_descend_stmt_tail eq_refl CallOk10)) as rhs.
+assert (G: lhs = rhs). { subst. apply IHlist10. apply TailOk. }
+now rewrite G.
+Qed.
+
+Lemma interpret_translated_stmt {C: VyperConfig}
+                                {bigger_call_depth_bound smaller_call_depth_bound: nat}
+                                (Ebound: bigger_call_depth_bound = S smaller_call_depth_bound)
+                                {cd: L10.Descend.calldag}
+                                (builtins: string -> option builtin)
+                                (fc: fun_ctx cd bigger_call_depth_bound)
+                                {cd2: L20.Descend.calldag}
+                                (ok: cd2 = translate_calldag cd)
+                                {do_call_10: forall
+                                      (fc': fun_ctx cd smaller_call_depth_bound)
+                                      (world: world_state)
+                                      (arg_values: list uint256),
+                                    world_state * expr_result uint256}
+                                {do_call_20: forall
+                                      (fc': fun_ctx cd2 smaller_call_depth_bound)
+                                      (world: world_state)
+                                      (arg_values: list uint256),
+                                    world_state * expr_result uint256}
+                                (DoCallOk: forall fc' world arg_values,
+                                             do_call_20 (translate_fun_ctx fc' ok) world arg_values
+                                              =
+                                             do_call_10 fc' world arg_values)
+                                (world: world_state)
+                                (loc: string_map uint256)
+                                {s10: L10.AST.stmt}
+                                {s20: L20.AST.stmt}
+                                (NotVarDecl: L10.AST.is_local_var_decl s10 = false)
+                                (StmtOk: s20 = let is_private_call := fun name: string =>
+                                                  match cd_declmap cd name with
+                                                  | Some _ => true
+                                                  | _ => false
+                                                  end
+                                               in translate_stmt is_private_call s10)
+                                (CallOk20: let _ := string_set_impl in 
+                                   FSet.is_subset (L20.Callset.stmt_callset s20)
+                                                  (L20.Callset.decl_callset
+                                                     (fun_decl
+                                                       (translate_fun_ctx fc ok)))
+                                   = true)
+                                (CallOk10: let _ := string_set_impl in 
+                                   FSet.is_subset (L10.Callset.stmt_callset s10)
+                                                  (L10.Callset.decl_callset
+                                                    (fun_decl fc))
+                                   = true):
+   L20.Stmt.interpret_stmt Ebound (translate_fun_ctx fc ok) do_call_20 builtins
+                           world loc s20 CallOk20
+    =
+   L10.Stmt.interpret_stmt Ebound fc do_call_10 builtins
+                           world loc s10 NotVarDecl CallOk10.
+Proof.
+subst bigger_call_depth_bound.
+(* Unfortunately, the inline fixpoints for interpret_stmt_list are not
+   the same as interpret_stmt_list from Coq's viewpoint.
+   All this is really stupid.
+ *)
+pose (is_private_call :=
+                 fun name : string => match cd_declmap cd name with
+                                      | Some _ => true
+                                      | None => false
+                                      end).
+pose (interpret_stmt_list' := fix
+   interpret_stmt_list (world0 : world_state) (loc0 : string_map uint256) (stmts : list L10.AST.stmt)
+                       (CallOk : FSet.is_subset (Callset.stmt_list_callset stmts)
+                                 (L10.Callset.decl_callset (fun_decl fc)) = true) {struct stmts} :
+   world_state * string_map uint256 * stmt_result uint256 :=
+   match
+     stmts as stmts' return (stmts = stmts' -> world_state * string_map uint256 * stmt_result uint256)
+   with
+   | nil => fun _ : stmts = nil => (world0, loc0, StmtSuccess)
+   | (h :: t)%list =>
+       fun E : stmts = (h :: t)%list =>
+       (if AST.is_local_var_decl h as h_is_var_decl
+         return
+           (AST.is_local_var_decl h = h_is_var_decl ->
+            world_state * string_map uint256 * stmt_result uint256)
+        then
+         fun Evar : AST.is_local_var_decl h = true =>
+         match map_lookup loc0 (fst (AST.var_decl_unpack h Evar)) with
+         | Some _ => (world0, loc0, StmtAbort (AbortError "local variable already exists"))
+         | None =>
+             match
+               snd (AST.var_decl_unpack h Evar) as init'
+               return
+                 (snd (AST.var_decl_unpack h Evar) = init' ->
+                  world_state * string_map uint256 * stmt_result uint256)
+             with
+             | Some init_expr =>
+                 fun Einit : snd (AST.var_decl_unpack h Evar) = Some init_expr =>
+                 match
+                   L10.Expr.interpret_expr eq_refl fc do_call_10 builtins world0 loc0 init_expr
+                     (Callset.callset_descend_init_expr E Evar Einit CallOk)
+                 with
+                 | (world', ExprSuccess value0) =>
+                     let
+                     '(world2, loc2, result2) :=
+                      interpret_stmt_list world0
+                        (map_insert loc0 (fst (AST.var_decl_unpack h Evar)) value0) t
+                        (Callset.callset_descend_stmt_tail E CallOk) in
+                      (world2, map_remove loc2 (fst (AST.var_decl_unpack h Evar)), result2)
+                 | (world', ExprAbort ab) => (world', loc0, StmtAbort ab)
+                 end
+             | None =>
+                 fun _ : snd (AST.var_decl_unpack h Evar) = None =>
+                 let
+                 '(world', loc', result) :=
+                  interpret_stmt_list world0 (map_insert loc0 (fst (AST.var_decl_unpack h Evar)) zero256)
+                    t (Callset.callset_descend_stmt_tail E CallOk) in
+                  (world', map_remove loc' (fst (AST.var_decl_unpack h Evar)), result)
+             end eq_refl
+         end
+        else
+         fun Evar : AST.is_local_var_decl h = false =>
+         match
+           L10.Stmt.interpret_stmt eq_refl fc do_call_10 builtins world0 loc0 h Evar
+             (Callset.callset_descend_stmt_head E CallOk)
+         with
+         | (world', loc', StmtSuccess) =>
+             interpret_stmt_list world' loc' t (Callset.callset_descend_stmt_tail E CallOk)
+         | (world', loc', StmtAbort _ as result) | (world', loc', StmtReturnFromFunction _ as result) =>
+             (world', loc', result)
+         end) eq_refl
+   end eq_refl).
+assert (interpret_stmt_list_alt: forall (w: world_state) 
+                                         (loc: string_map uint256)
+                                         (l: list L10.AST.stmt)
+                                         (LCallOk: let _ := string_set_impl in
+                                                   FSet.is_subset
+                                                     (Callset.stmt_list_callset l)
+                                                     (L10.Callset.decl_callset (fun_decl fc))
+                                                   = true),
+   interpret_stmt_list' w loc l LCallOk
+    =
+   L10.Stmt.interpret_stmt_list eq_refl fc do_call_10 builtins w loc l LCallOk).
+{
+  clear world loc NotVarDecl s10 s20 StmtOk CallOk10 CallOk20.
+  intros w loc l. revert w loc.
+  induction l. { easy. }
+  cbn. intros.
+  remember (fun Evar : AST.is_local_var_decl a = false =>
+              match
+                L10.Stmt.interpret_stmt eq_refl fc do_call_10 builtins w loc a Evar
+                  (Callset.callset_descend_stmt_head eq_refl LCallOk)
+              with
+              | (world', loc', StmtSuccess) =>
+                  interpret_stmt_list' world' loc' l
+                    (Callset.callset_descend_stmt_tail eq_refl LCallOk)
+              | (world', loc', StmtAbort _ as result) | (world', loc', StmtReturnFromFunction _ as result) =>
+                  (world', loc', result)
+              end) as not_var_branch1.
+  remember (fun Evar : AST.is_local_var_decl a = false =>
+              match
+                L10.Stmt.interpret_stmt eq_refl fc do_call_10 builtins w loc a Evar
+                  (Callset.callset_descend_stmt_head eq_refl LCallOk)
+              with
+              | (world', loc', StmtSuccess) =>
+                  L10.Stmt.interpret_stmt_list eq_refl fc do_call_10 builtins world' loc' l
+                    (Callset.callset_descend_stmt_tail eq_refl LCallOk)
+              | (world', loc', StmtAbort _ as result) | (world', loc', StmtReturnFromFunction _ as result) =>
+                  (world', loc', result)
+              end) as not_var_branch2.
+  assert (B: forall (Evar: AST.is_local_var_decl a = false),
+               not_var_branch1 Evar = not_var_branch2 Evar).
+  {
+    subst. intro Evar.
+    L10.Expr.destruct_let_pair. destruct p. now destruct s.
+  }
+  clear Heqnot_var_branch1 Heqnot_var_branch2.
+  destruct a; try easy.
+  (* local var *)
+  cbn.
+  destruct map_lookup. { trivial. }
+  destruct init. 2:{ now rewrite IHl. }
+  destruct L10.Expr.interpret_expr.
+  destruct e0. { now rewrite IHl. }
+  trivial.
+} (* interpret_stmt_list_alt *)
+subst cd2.
+(* Another round of stupidity: we also need to fold translate_stmt_list. *)
+pose (translate_stmt_list' := fix translate_stmt_list (l : list L10.AST.stmt) : AST.stmt :=
+                 match l with
+                 | nil => AST.SmallStmt AST.Pass
+                 | (L10.AST.LocalVarDecl name maybe_init :: t)%list =>
+                     AST.LocalVarDecl name
+                       match maybe_init with
+                       | Some init =>
+                           translate_expr
+                             (fun name0 : string =>
+                              match cd_declmap cd name0 with
+                              | Some _ => true
+                              | None => false
+                              end) init
+                       | None => AST.Const zero256
+                       end (translate_stmt_list t)
+                 | (L10.AST.SmallStmt _ as h :: t)%list | (L10.AST.IfElseStmt _ _ _ as h :: t)%list |
+                   (AST.FixedRangeLoop _ _ _ _ as h :: t)%list |
+                   (AST.FixedCountLoop _ _ _ _ as h :: t)%list =>
+                     AST.Semicolon
+                       (translate_stmt
+                          (fun name : string =>
+                           match cd_declmap cd name with
+                           | Some _ => true
+                           | None => false
+                           end) h) (translate_stmt_list t)
+                 end).
+assert (translate_stmt_list_alt: forall l: list L10.AST.stmt,
+          translate_stmt_list' l  =  translate_stmt_list is_private_call l).
+{ now induction l. }
+pose (AllOk := (* all statements in the given list of statements translate correctly *)
+         List.Forall
+             (fun s : L10.AST.stmt =>
+              let is_private_call :=
+                fun name : string => match cd_declmap cd name with
+                                     | Some _ => true
+                                     | None => false
+                                     end in
+              forall (NotVarDecl0 : AST.is_local_var_decl s = false)
+                (CallOk21 : let H := string_set_impl in
+                            FSet.is_subset (Callset.stmt_callset (translate_stmt is_private_call s))
+                              (Callset.decl_callset (fun_decl (translate_fun_ctx fc eq_refl))) = true)
+                (CallOk11 : let H := string_set_impl in
+                            FSet.is_subset (L10.Callset.stmt_callset s) (L10.Callset.decl_callset (fun_decl fc)) =
+                            true) (world0 : world_state) (loc0 : string_map uint256),
+              L20.Stmt.interpret_stmt eq_refl (translate_fun_ctx fc eq_refl) do_call_20 builtins world0 loc0
+                (translate_stmt is_private_call s) CallOk21 =
+              L10.Stmt.interpret_stmt eq_refl fc do_call_10 builtins world0 loc0 s NotVarDecl0 CallOk11)).
+revert world loc. subst s20.
+assert (P: cached_translated_decl fc eq_refl = fun_decl (translate_fun_ctx fc eq_refl)).
+{ unfold translate_fun_ctx. now subst. }
+induction s10 using L10.AST.stmt_ind'; intros.
+{ (* small *) now apply interpret_translated_small_stmt. }
+{ (* local var *) cbn in NotVarDecl. discriminate. }
+{ (* if *)
+  cbn.
+  expr. L10.Expr.destruct_let_pair.
+  destruct e. 2:{ trivial. }
+  destruct (Z_of_uint256 value =? 0)%Z.
+  { (* else *)
+    destruct no. 2:easy.
+
+    assert (G: let _ := string_set_impl in
+               FSet.is_subset (Callset.stmt_callset (translate_stmt_list is_private_call l))
+                 (Callset.decl_callset (fun_decl (translate_fun_ctx fc eq_refl))) = true).
+    { rewrite<- P. apply (L20.Callset.callset_descend_stmt_if_else eq_refl CallOk20). }
+
+    assert (L: AllOk l).
+    {
+      unfold AllOk.
+      rewrite List.Forall_forall.
+      rewrite List.Forall_forall in H0.
+      intros.
+      now apply H0. (* why can't it just apply it directly? *)
+    }
+    mark.
+    assert (W := weak_stmt_list_ok eq_refl builtins fc DoCallOk w loc
+                 G
+                 (L10.Callset.callset_descend_stmt_if_else eq_refl eq_refl CallOk10)
+                 L).
+    assert (E: G = L20.Callset.callset_descend_stmt_if_else eq_refl CallOk20).
+    { apply PropExtensionality.proof_irrelevance. }
+    rewrite E in W.
+    assert (T := eq_trans Heqlhs W). (* why rewrite W doesn't work? *)
+    clear Heqlhs. subst.
+    rewrite interpret_stmt_list_alt.
+    trivial.
+  }
+  (* then *)
+  assert (G: let _ := string_set_impl in
+           FSet.is_subset (Callset.stmt_callset (translate_stmt_list is_private_call yes))
+             (Callset.decl_callset (fun_decl (translate_fun_ctx fc eq_refl))) = true).
+  { rewrite<- P. apply (L20.Callset.callset_descend_stmt_if_then eq_refl CallOk20). }
+  assert (L: AllOk yes).
+  {
+    unfold AllOk.
+    rewrite List.Forall_forall.
+    rewrite List.Forall_forall in H.
+    intros.
+    now apply H. (* why can't it just apply it directly? *)
+  }
+  mark.
+  assert (W := weak_stmt_list_ok eq_refl builtins fc DoCallOk w loc
+               G
+               (L10.Callset.callset_descend_stmt_if_then eq_refl CallOk10)
+               L).
+  assert (E: G = L20.Callset.callset_descend_stmt_if_then eq_refl CallOk20).
+  { apply PropExtensionality.proof_irrelevance. }
+  rewrite E in W.
+  assert (T := eq_trans Heqlhs W). (* why rewrite W doesn't work? *)
+  clear Heqlhs. subst.
+  rewrite interpret_stmt_list_alt.
+  trivial.
+}
+2:{ (* fixed count loop *)
+  cbn. expr.
+  destruct (map_lookup loc var). { trivial. }
+  L10.Expr.destruct_let_pair. destruct e. 2:{ trivial. }
+  remember
+    (Z_of_uint256 (uint256_of_Z (Z_of_uint256 value + Z_of_uint256 count - 1)) 
+     =? 
+    Z_of_uint256 value + Z_of_uint256 count - 1)%Z as overflow_check.
+  destruct overflow_check. 2:{ trivial. }
+  remember (Z.to_nat (Z_of_uint256 count)) as n.
+  remember (Z_of_uint256 value + Z_of_uint256 count - 1)%Z as cap.
+
+  (* Here Heqcap is the main loop equation: [
+
+        cap = Z_of_uint256 value + Z_of_uint256 count - 1
+
+    ] where cap is constant, value goes up and count goes down.
+  However, in our interpretation of the count loop we allow overflow
+  during the last iteration, for example [
+
+      for i in count(2^256 - 2, 2):
+        ...
+
+  ] is the same as [
+
+      for i in [2^256 - 2, 2^256 - 1]:
+        ...
+  ] and therefore legit (except that the latter syntax is currently 
+  not supported). Therefore the main loop equation must be weakened to this: *)
+  assert (WeakMainLoopEq: 
+            cap = (Z_of_uint256 value + Z_of_uint256 count - 1)%Z
+             \/
+            Z_of_uint256 count = 0%Z).
+  { left. exact Heqcap. }
+  clear Heqcap.
+  revert count NotVarDecl CallOk10 CallOk20 Heqn w loc value WeakMainLoopEq.
+  induction n. { easy. }
+  intros.
+
+  (* checking that the counter doesn't go below 0 *)
+  pose (count' := uint256_of_Z (Z.pred (Z_of_uint256 count))).
+  assert (CountOk: n = Z.to_nat (Z_of_uint256 count')).
+  {
+    unfold count'. rewrite uint256_ok.
+    assert (R := uint256_range count).
+    remember (Z_of_uint256 count) as z. clear Heqz.
+    assert (Q: z = Z.succ (Z.of_nat n)).
+    {
+      rewrite<- Nat2Z.inj_succ. rewrite Heqn.
+      symmetry. apply Z2Nat.id. tauto.
+    }
+    subst z. rewrite Z.pred_succ.
+    replace (Z.of_nat n mod 2 ^ 256)%Z with (Z.of_nat n).
+    { symmetry. apply Nat2Z.id. }
+    symmetry. apply Z.mod_small.
+    split.
+    { (* 0 <= n *) apply Nat2Z.is_nonneg. }
+    exact (Z.lt_trans _ _ _ (Z.lt_succ_diag_r (Z.of_nat n)) (proj2 R)).
+  }
+
+  assert (G: let _ := string_set_impl in
+             FSet.is_subset (Callset.stmt_callset (translate_stmt_list is_private_call body))
+               (Callset.decl_callset (fun_decl (translate_fun_ctx fc eq_refl))) = true).
+  { rewrite<- P. apply (L20.Callset.callset_descend_loop_body eq_refl CallOk20). }
+
+  assert (L: AllOk body).
+  {
+    unfold AllOk.
+    rewrite List.Forall_forall.
+    rewrite List.Forall_forall in H.
+    intros.
+    now apply H.
+  }
+  mark.
+  assert (W := weak_stmt_list_ok eq_refl builtins fc DoCallOk w
+               (map_insert loc var (uint256_of_Z (Z_of_uint256 value)))
+               G
+               (L10.Callset.callset_descend_fixed_count_loop_body eq_refl CallOk10)
+               L).
+  fold is_private_call in W. 
+  fold translate_stmt_list' in Heqlhs.
+  rewrite interpret_stmt_list_alt in Heqrhs.
+  destruct L10.Stmt.interpret_stmt_list as ((world', loc'), result').
+
+  (* This hairball is copied from Heqlhs.
+     It looks like [
+          Stmt.interpret_stmt eq_refl (translate_fun_ctx fc eq_refl) do_call_20 builtins w
+              (map_insert loc var (uint256_of_Z (Z_of_uint256 value)))
+              (translate_stmt_list' body)
+              (Callset.callset_descend_loop_body eq_refl CallOk20)
+    ] but if I write just that then it doesn't match. *)
+  assert (V: @Stmt.interpret_stmt C (S smaller_call_depth_bound) smaller_call_depth_bound
+             (@eq_refl nat (S smaller_call_depth_bound)) (@translate_calldag C cd)
+             (@translate_fun_ctx C (S smaller_call_depth_bound) cd fc (@translate_calldag C cd)
+                (@eq_refl (@Descend.calldag C) (@translate_calldag C cd))) do_call_20 builtins w
+             (@map_insert C (@uint256 C) loc var (@uint256_of_Z C (@Z_of_uint256 C value)))
+             (translate_stmt_list' body)
+             (@Callset.callset_descend_loop_body C
+                (@AST.Loop C var
+                   (@translate_expr C
+                      (fun name : string =>
+                       match @cd_declmap C (@L10.AST.decl C) (@L10.Callset.decl_callset C) cd name with
+                       | Some _ => true
+                       | None => false
+                       end) start) count (translate_stmt_list' body)) (translate_stmt_list' body) var
+                (@translate_expr C
+                   (fun name : string =>
+                    match @cd_declmap C (@L10.AST.decl C) (@L10.Callset.decl_callset C) cd name with
+                    | Some _ => true
+                    | None => false
+                    end) start) count
+                (@Callset.decl_callset C
+                   (@cached_translated_decl C (S smaller_call_depth_bound) cd fc 
+                      (@translate_calldag C cd) (@eq_refl (@Descend.calldag C) (@translate_calldag C cd))))
+                (@eq_refl (@AST.stmt C)
+                   (@AST.Loop C var
+                      (@translate_expr C
+                         (fun name : string =>
+                          match @cd_declmap C (@L10.AST.decl C) (@L10.Callset.decl_callset C) cd name with
+                          | Some _ => true
+                          | None => false
+                          end) start) count (translate_stmt_list' body))) CallOk20)
+             = (world', loc', result')).
+  {
+    assert (E: G = L20.Callset.callset_descend_loop_body eq_refl CallOk20).
+    { apply PropExtensionality.proof_irrelevance. }
+    rewrite E in W.
+    apply W.
+  }
+  rewrite V in Heqlhs.
+  clear V W G.
+
+  assert (CapRange: (0 <= cap < 2 ^ 256)%Z).
+  {
+    symmetry in Heqoverflow_check. rewrite Z.eqb_eq in Heqoverflow_check.
+    rewrite uint256_ok in Heqoverflow_check.
+    rewrite Z.mod_small_iff in Heqoverflow_check by apply two_to_256_ne_0.
+    enough (~ (2 ^ 256 < cap <= 0)%Z). { tauto. }
+    intro Y.
+    assert (Bad := proj2 (Z.ltb_lt _ _) (Z.lt_le_trans _ _ _ (proj1 Y) (proj2 Y))).
+    cbn in Bad. discriminate.
+  }
+
+  assert (MainLoopEq: cap = (Z_of_uint256 value + Z_of_uint256 count - 1)%Z).
+  {
+    enough (Z_of_uint256 count <> 0%Z). { tauto. }
+    intro J. rewrite J in *.
+    cbn in Heqn. discriminate.
+  }
+
+  pose (value' := uint256_of_Z (Z.succ (Z_of_uint256 value))).
+  assert (NextWeakMainLoopEq:
+     cap = (Z_of_uint256 value' + Z_of_uint256 count' - 1)%Z 
+      \/
+     Z_of_uint256 count' = 0%Z).
+  {
+    unfold value'.
+    rewrite uint256_ok.
+    destruct n.
+    {
+      (* CountOk: 0 = Z.to_nat (Z_of_uint256 count') *)
+      right.
+      assert (Y: Z.of_nat (Z.to_nat (Z_of_uint256 count')) = 0%Z)
+        by now rewrite<- CountOk.
+      rewrite Z2Nat.id in Y. { exact Y. }
+      exact (proj1 (uint256_range count')).
+    }
+    left.
+    assert (ValueOk: Z_of_uint256 value' = Z.succ (Z_of_uint256 value)).
+    {
+      unfold value'.
+      rewrite uint256_ok.
+      apply Z.mod_small.
+      subst cap.
+      split.
+      { (* 0 <= Z.succ (Z_of_uint256 value)) *)
+        apply Z.le_le_succ_r.
+        apply (proj1 (uint256_range _)).
+      }
+      (* Heqn: S (S n) = Z.to_nat (Z_of_uint256 count) *)
+      lia.
+    }
+    rewrite<- ValueOk.
+    replace (Z_of_uint256 value' mod 2 ^ 256)%Z with (Z_of_uint256 value').
+    2:{ symmetry. apply Z.mod_small. apply uint256_range. }
+    rewrite MainLoopEq.
+    f_equal.
+    rewrite ValueOk.
+    assert (CountOk': Z_of_uint256 count' = Z.pred (Z_of_uint256 count)).
+    {
+      replace (Z_of_uint256 count') with (Z.of_nat (S n)).
+      2:{
+        rewrite CountOk. rewrite Z2Nat.id. { trivial. }
+        exact (proj1 (uint256_range count')).
+      }
+      replace (Z_of_uint256 count) with (Z.of_nat (S (S n))).
+      2:{
+        rewrite Heqn. rewrite Z2Nat.id. { trivial. }
+        exact (proj1 (uint256_range count)).
+      }
+      lia.
+    }
+    rewrite CountOk'.
+    lia.
+  }
+
+  (* Fix invisible problems in the induction hypothesis:
+      IHn' arrives to the callset of the body via a loop with count',
+      but the goal arrives to the same via a loop with count.
+     *)
+
+  assert (FixCount20: @L20.Callset.callset_descend_loop_body C
+              (@AST.Loop C var
+                 (@translate_expr C
+                    (fun name : string =>
+                     match
+                       @cd_declmap C (@L10.AST.decl C) (@L10.Callset.decl_callset C) cd name
+                     with
+                     | Some _ => true
+                     | None => false
+                     end) start) count' (translate_stmt_list' body)) (translate_stmt_list' body)
+              var
+              (@translate_expr C
+                 (fun name : string =>
+                  match @cd_declmap C (@L10.AST.decl C) (@L10.Callset.decl_callset C) cd name with
+                  | Some _ => true
+                  | None => false
+                  end) start) count'
+              (@Callset.decl_callset C
+                 (@cached_translated_decl C (S smaller_call_depth_bound) cd fc
+                    (@translate_calldag C cd)
+                    (@eq_refl (@Descend.calldag C) (@translate_calldag C cd))))
+              (@eq_refl (@AST.stmt C)
+                 (@AST.Loop C var
+                    (@translate_expr C
+                       (fun name : string =>
+                        match
+                          @cd_declmap C (@L10.AST.decl C) (@L10.Callset.decl_callset C) cd name
+                        with
+                        | Some _ => true
+                        | None => false
+                        end) start) count' (translate_stmt_list' body))) CallOk20
+            = Callset.callset_descend_loop_body eq_refl CallOk20).
+  { apply PropExtensionality.proof_irrelevance. }
+
+  assert (FixCount10: @L10.Callset.callset_descend_fixed_count_loop_body C
+                       (@AST.FixedCountLoop C var start count' body) body var start count'
+                       (@L10.Callset.decl_callset C
+                          (@fun_decl C (@L10.AST.decl C) (@L10.Callset.decl_callset C) cd
+                             (S smaller_call_depth_bound) fc))
+                       (@eq_refl (@L10.AST.stmt C) (@AST.FixedCountLoop C var start count' body))
+                       CallOk10
+                     =
+                    L10.Callset.callset_descend_fixed_count_loop_body eq_refl CallOk10).
+  { apply PropExtensionality.proof_irrelevance. }
+
+  fold interpret_stmt_list'.
+  fold interpret_stmt_list' in IHn.
+  fold translate_stmt_list' in IHn.
+
+  destruct result'; subst lhs rhs. 3:{ trivial. }
+  { (* successful iteration *)
+    assert (IHn' := IHn count' eq_refl CallOk10 CallOk20 CountOk 
+                        world' loc' value' NextWeakMainLoopEq).
+    rewrite FixCount10 in IHn'.
+    rewrite FixCount20 in IHn'.
+
+    assert (NZ: n = 0 \/ n <> 0) by lia.
+    destruct NZ. { now destruct n. }
+    (* XXX dup from above *)
+    assert (ValueOk: Z_of_uint256 value' = Z.succ (Z_of_uint256 value)).
+    {
+      unfold value'.
+      rewrite uint256_ok.
+      apply Z.mod_small.
+      subst cap.
+      split.
+      { (* 0 <= Z.succ (Z_of_uint256 value)) *)
+        apply Z.le_le_succ_r.
+        apply (proj1 (uint256_range _)).
+      }
+      (* Heqn: S (S n) = Z.to_nat (Z_of_uint256 count) *)
+      lia.
+    }
+    rewrite<- ValueOk.
+    apply IHn'.
+  }
+  (* abort *)
+  destruct a; try easy.
+  (* continue (XXX dup from above) *)
+  assert (IHn' := IHn count' eq_refl CallOk10 CallOk20 CountOk 
+                        world' loc' value' NextWeakMainLoopEq).
+  rewrite FixCount10 in IHn'.
+  rewrite FixCount20 in IHn'.
+
+  assert (NZ: n = 0 \/ n <> 0) by lia.
+  destruct NZ. { now destruct n. }
+  (* XXX dup from above *)
+  assert (ValueOk: Z_of_uint256 value' = Z.succ (Z_of_uint256 value)).
+  {
+    unfold value'.
+    rewrite uint256_ok.
+    apply Z.mod_small.
+    subst cap.
+    split.
+    { (* 0 <= Z.succ (Z_of_uint256 value)) *)
+      apply Z.le_le_succ_r.
+      apply (proj1 (uint256_range _)).
+    }
+    (* Heqn: S (S n) = Z.to_nat (Z_of_uint256 count) *)
+    lia.
+  }
+  rewrite<- ValueOk.
+  apply IHn'.
+}
+(* fixed range loop *)
+cbn. destruct (map_lookup loc var). { trivial. }
+fold interpret_stmt_list'. fold translate_stmt_list'.
+remember (match start with
+          | Some x => x
+          | None => zero256
+          end) as start256.
+
+
+
+L10.Expr.destruct_let_pair. destruct e. 2:{ trivial. }
+remember
+  (Z_of_uint256 (uint256_of_Z (Z_of_uint256 value + Z_of_uint256 count - 1)) 
+   =? 
+  Z_of_uint256 value + Z_of_uint256 count - 1)%Z as overflow_check.
+destruct overflow_check. 2:{ trivial. }
+remember (Z.to_nat (Z_of_uint256 count)) as n.
+remember (Z_of_uint256 value + Z_of_uint256 count - 1)%Z as cap.
+
+(*
 
 
 Theorem interpret_translated_call {C: VyperConfig}
